New chaos

ntor/Metareduction.ec
@@ -1,6 +1,6 @@
 require import AllCore FSet FMap Distr DProd List SplitRO NTOR Games.
 (*   *) import GAKEc HROc.
-require (*  *) DiffieHellman.
+require (*  *) GAKE_nosid DiffieHellman.
 (*   *) import StdBigop.Bigreal.BRA StdOrder.RealOrder DH.G DH.GP DH.FD DH.GP.ZModE.
 
 (* ------------------------------------------------------------------------------------------ *)
@@ -11,6 +11,20 @@ require (*  *) DiffieHellman.
 (* Modified rondom oracle *)
 type pr_st_client_mod = pkey * skey.
 type pr_st_server_mod = skey * skey option.
+
+op rem_sid_c (s : pr_st_client instance_state) : pr_st_client_mod instance_state =
+match s with 
+| Pending st pt ir => Pending (st.`2, st.`3) pt ir
+| Accepted st t k ir => Accepted (st.`2, st.`3) t k ir
+| Aborted st t ir => Aborted (Some ((oget st).`2, (oget st).`3)) t ir
+end.
+
+op rem_sid_s (s : pr_st_server instance_state) : pr_st_server_mod instance_state =
+match s with 
+| Pending st pt ir => Pending (st.`2, st.`3) pt ir
+| Accepted st t k ir => Accepted (st.`2, st.`3) t k ir
+| Aborted st t ir => Aborted (Some ((oget st).`2, (oget st).`3)) t ir
+end.
 
 type h_mod_input = pkey * pkey * pkey * pkey * pkey.
 
@@ -86,686 +100,6 @@ module NTOR_C_mod (H : RO) : Client_mod = {
     return r;
   }
 }.
-
-(********************************************************************************)
-(* helping operators for getting a set of all partners (with some specific revealed status *)
-op get_partners_mod_c (t: trace) (fmap: (pkey * int, pr_st_server_mod instance_state) fmap) : (pkey * int) fset =
-fdom (
-  filter
-  (fun bj (val: pr_st_server_mod instance_state) =>
-       get_trace val = Some t (* Partners share the same trace *)
-  )
-  fmap
-).
-
-op get_partners_mod_s (t: trace) (fmap: (int, pr_st_client_mod instance_state) fmap) : int fset =
-fdom (
-  filter
-  (fun i (val: pr_st_client_mod instance_state) =>
-       get_trace val = Some t (* Partners share the same trace *)
-  )
-  fmap
-).
-
-op get_origins_mod_c (t: trace) (fmap: (pkey * int, pr_st_server_mod instance_state) fmap) : (pkey * int) fset =
-fdom (
-  filter
-  (fun bj (val: pr_st_server_mod instance_state) =>
-       (exists m2o, get_trace val = Some (fst t, m2o)) (* Partners share the same (partial) trace *)
-  )
-  fmap
-).
-
-op get_origins_mod_s (t: trace) (fmap: (int, pr_st_client_mod instance_state) fmap) : int fset =
-fdom (
-  filter
-  (fun i (val: pr_st_client_mod instance_state) =>
-       (exists m2o, get_trace val = Some (fst t, m2o)) (* Partners share the same (partial) trace *)
-  )
-  fmap
-).
-
-op get_untested_partners_mod_c (t: trace) (fmap: (pkey * int, pr_st_server_mod instance_state) fmap) : (pkey * int) fset =
-fdom (
-  filter
-  (fun bj (val: pr_st_server_mod instance_state) =>
-       get_trace val = Some t  (* Partners share the same trace *)
-    /\ get_ir_test val = false (* Partner is not tested *)
-  )
-  fmap
-).
-
-op get_untested_partners_mod_s (t: trace) (fmap: (int, pr_st_client_mod instance_state) fmap) : int fset =
-fdom (
-  filter
-  (fun i (val: pr_st_client_mod instance_state) =>
-       get_trace val = Some t  (* Partners share the same trace *)
-    /\ get_ir_test val = false (* Partner is not tested *)
-  )
-  fmap
-).
-
-op get_untested_origins_mod_c (t: trace) (fmap: (pkey * int, pr_st_server_mod instance_state) fmap) : (pkey * int) fset =
-fdom (
-  filter
-  (fun bj (val: pr_st_server_mod instance_state) =>
-       (exists m2o, get_trace val = Some (fst t, m2o)) (* Partners share the same (partial) trace *)
-    /\ get_ir_test val = false                         (* Partner is not tested *)
-  )
-  fmap
-).
-
-
-op get_fresh_partners_mod_c (t: trace) (fmap1: (pkey * int, pr_st_server_mod instance_state) fmap) (fmap2: (pkey, skey option) fmap) : (pkey * int) fset =
-fdom (
-  filter
-  (fun bj (val: pr_st_server_mod instance_state) =>
-       get_trace val = Some t                                    (* Partners share the same trace *)
-    /\ get_ir_test val = false                                   (* Partner is not tested *)
-    /\ get_ir_sess val = false                                   (* Partner is not revealed *)
-    /\ (get_ir_eph val = false \/ (oget fmap2.[fst bj]) <> None) (* Partner is not trivially broken *)
-  )
-  fmap1
-).
-
-(* since ephkey reveal is permitted on Pending client instances we need to consider partial traces for partnering *)
-op get_fresh_partners_mod_s (t : trace) (fmap: (int, pr_st_client_mod instance_state) fmap) : int fset =
-fdom (
-  filter
-  (fun i (val: pr_st_client_mod instance_state) =>
-       (* CHECK: we consider *any* client that has sent this first message to be a pre-partner *)
-       (exists m2o, get_trace val = Some (fst t, m2o)) (* Partners share the same (partial) trace *)
-    /\ get_ir_test val = false                         (* Partner is not tested *)
-    /\ get_ir_sess val = false                         (* Partner is not revealed *)
-    /\ get_ir_eph val = false                          (* Partner is not trivially broken *)
-  )
-  fmap
-).
-
-(* operators that return None if there is no partner, true if there is an untested/fresh partner or false if all partners are tested/unfresh *)
-op untested_origins_mod_c (t: trace) (fmap: (pkey * int, pr_st_server_mod instance_state) fmap) : bool option =
-if 1 <= card (get_origins_mod_c t fmap) then Some (1 <= card (get_untested_origins_mod_c t fmap)) else None.
-
-op untested_partner_mod_c (t: trace) (fmap: (pkey * int, pr_st_server_mod instance_state) fmap) : bool option =
-if 1 <= card (get_partners_mod_c t fmap) then Some (1 <= card (get_untested_partners_mod_c t fmap)) else None.
-
-op fresh_partner_mod_c (t: trace) (fmap1: (pkey * int, pr_st_server_mod instance_state) fmap) (fmap2: (pkey, skey option) fmap) : bool option =
-if 1 <= card (get_origins_mod_c t fmap1) then Some (1 <= card (get_fresh_partners_mod_c t fmap1 fmap2)) else None.
-
-op untested_partner_mod_s (t: trace) (fmap: (int, pr_st_client_mod instance_state) fmap) : bool option =
-if 1 <= card (get_partners_mod_s t fmap) then Some (1 <= card (get_untested_partners_mod_s t fmap)) else None.
-
-op fresh_partner_mod_s (t: trace) (fmap: (int, pr_st_client_mod instance_state) fmap) : bool option =
-if 1 <= card (get_origins_mod_s t fmap) then Some (1 <= card (get_fresh_partners_mod_s t fmap)) else None.
-
-
-(* Modified GAKE game *)
-module type GAKE_mod_out = {
-  proc h(input: h_mod_input) : tag * key
-
-  proc init_s() : pkey
-  proc set_cert(pk: pkey) : unit option
-
-  proc send_msg1(i: int, m1: pkey) : pkey option
-  proc send_msg2(b: pkey, j: int, m2: pkey) : (pkey * tag) option
-
-  proc s_rev_skey(b: pkey, j: int) : key option
-  proc rev_ltkey(b: pkey) : skey option
-  proc s_rev_ephkey(b: pkey, j: int) : skey option
-  proc s_test(b: pkey, j: int) : key option
-
-  include GAKE_out [send_msg3, c_rev_skey, c_rev_ephkey, c_test]
-}.
-
-module type GAKE_mod_out_i = {
-  include GAKE_mod_out
-
-  proc init_mem(b : bool) : unit
-}.
-
-module GAKEb_mod (S: Server_mod) (C: Client_mod) (H : RO) : GAKE_mod_out = {
-  var b0 : bool 
-
-  var s_kp : (pkey, skey option) fmap
-  var c_smap : (int, pr_st_client_mod instance_state) fmap
-  var s_smap : (pkey * int, pr_st_server_mod instance_state) fmap
-  
-  var tested : int option
-
-  proc init_mem(b: bool) : unit = {
-    b0 <- b;
-    H.init();
-    s_kp <- empty;
-    c_smap <- empty;
-    s_smap <- empty;
-    tested <- None;
-  }
-
-  (* random oracle *)
-  proc h = H.get
-  
-  (* server management *)
-  proc init_s() : pkey = {
-    var kp;
-
-    kp <@ S.keygen();
-    s_kp.[kp.`1] <- Some kp.`2;
-
-    return kp.`1;
-  }
-
-  proc set_cert(pk: pkey) : unit option = {
-    var r <- None;
-
-    s_kp.[pk] <- None;
-    r <- Some ();
-
-    return r;
-  }
-
-  proc send_msg1(i: int, m1: pkey) : pkey option = {
-    var st, st', m2;
-    var r <- None;
-
-    st <- c_smap.[i];
-    if (m1 \in s_kp) {
-      match st with
-      | None => {
-          (st', m2) <@ C.new_session(m1);
-           c_smap.[i] <- Pending st' m2 (false, false, false);
-          r <- Some m2;
-        }
-      | Some st => {
-          match st with
-          | Pending st pt ir => c_smap.[i] <- Aborted (Some st) (Some (pt, None)) ir;
-          | Accepted _ _ _ _ => { }
-          | Aborted _ _ _ => { }
-          end;
-        }
-      end;
-    }
-    return r;
-  }
-
-  proc send_msg2(b: pkey, j: int, m2: pkey) : (pkey * tag) option = {
-    var sko, resp, st', k, m3;
-    var r <- None;
-
-    sko <- oget s_kp.[b];
-    if (sko is Some sk) (* Server was initialised as honest *) {
-      match s_smap.[b, j] with
-      | None => {
-          resp <@ S.respond_session(Some (sk, None), m2);
-          if (resp is Some r') {
-            (st', m3, k) <- r';
-            s_smap.[(b, j)] <- Accepted st' (m2, Some m3) k (false, false, false);
-            r <- Some m3;
-          } else {
-            s_smap.[(b, j)] <- Aborted None (Some (m2, None)) (false, false, false);
-          }
-        }
-      | Some st => { (* only completed sessions would be stored, and those can't be aborted; do nothing *) }
-      end;
-    }
-
-    return r;
-  }
-
-  proc send_msg3(i: int, m3: pkey * tag) : unit option = {
-    var resp, st', k;
-    var r <- None;
-
-    match c_smap.[i] with
-    | None => { } (* Abort? *)
-    | Some st => {
-        match st with
-        | Pending st pt ir => {
-            resp <@ C.complete_session(st, m3);
-            if (resp is Some r') {
-              (st', k) <- r';
-              c_smap.[i] <- Accepted st' (pt, Some m3) k ir;
-              r <- Some ();
-            } else {
-              c_smap.[i] <- Aborted (Some st) (Some (pt, Some m3)) ir;
-            }
-          }
-        | Accepted _ _ _ _ => { }
-        | Aborted _ _ _ => { }
-        end;
-      }
-    end;
-    return r;
-  }
-
-
-  (* reveal and test *)
-  proc c_rev_skey(i: int) : key option = {
-    var k <- None;
-
-    match c_smap.[i] with
-    | None => { }
-    | Some st => {
-        (* only accepted client instances that are not tested and 
-           that not only have tested partners can be sesskey revealed *)
-        if (st is Accepted st' t' k' ir') {
-          if (!(get_ir_test (oget c_smap.[i]) \/ untested_partner_mod_c t' s_smap = Some false)) {
-            k <- Some k';
-            c_smap.[i] <- set_ir_sess (Accepted st' t' k' ir');
-          }
-        }
-      }
-    end;
-    return k;
-  }
-
-  proc s_rev_skey(b: pkey, j: int) : key option = {
-    var k <- None;
-
-    match s_smap.[(b, j)] with
-    | None => { }
-    | Some st => {
-        (* only accepted server instances that are not tested and 
-           that not only have tested partners can be sesskey revealed *)
-        if (st is Accepted st' t' k' ir') {
-          if (!(get_ir_test (oget s_smap.[b, j]) \/ untested_partner_mod_s t' c_smap = Some false)) {
-            k <- Some k';
-            s_smap.[(b, j)] <- set_ir_sess (Accepted st' t' k' ir');
-          }
-        }
-      }
-    end;
-    return k;
-  }
-
-  proc rev_ltkey(b: pkey) : skey option = {
-    var ltk <- None;
-
-    match s_kp.[b] with
-    | None => { }
-    | Some sk => {
-        (* a server can be ltkey revealed if no instance of it is ephkey revealed 
-           in case that instance or all its partners are tested *) 
-        if (forall j,
-              (b, j) \in s_smap (* just checking instances of b *)
-              => !(   (   get_ir_test (oget s_smap.[b, j])
-                          (* This is always OK (get_trace always Some on server side *)
-                       \/ untested_partner_mod_s (oget (get_trace (oget s_smap.[b, j]))) c_smap = Some false)
-                   /\ get_ir_eph (oget s_smap.[b,j]))) {
-          ltk <- sk; 
-      (*    servers.[b] <- Corrupt kp; *)
-          s_kp.[b] <- None; 
-        }
-      }
-    end;
-    return ltk;
-  }
-
-  proc c_rev_ephkey(i: int) : skey option = {
-    var ek <- None;
-
-    match c_smap.[i] with
-    | None => { }
-    | Some st => {
-        match st with
-          (* client instances can be ephkey revealed when pending if there isn't 
-             a tested origin partner (agreeing on first message *)
-        | Pending st pk_e ir => {
-            if (untested_origins_mod_c (pk_e, None) s_smap <> Some false) {
-              ek <- Some (st.`2);
-              c_smap.[i] <- set_ir_eph (Pending st pk_e ir);
-            }
-          }
-          (* accepted client instamces can only be ephkey revealed when not tested and 
-             if not all partners are tested *)
-        | Accepted st t k ir => {
-            if (!(get_ir_test (oget c_smap.[i]) \/ untested_partner_mod_c t s_smap = Some false)) {
-              ek <- Some (st.`2);
-              c_smap.[i] <- set_ir_eph (Accepted st t k ir);
-            }
-          }
-        | Aborted _ _ _ => {  }
-        end;
-      }
-    end;
-    return ek;
-  }
-
-  proc s_rev_ephkey(b: pkey, j: int) : skey option = {
-    var ek <- None;
-
-    match s_smap.[b, j] with
-    | None => { }
-    | Some st => {
-        (* only accepted server instances that are not ltkey revealed in case they 
-           or all partners are tested can be ephkey revealed *)
-        if (st is Accepted st t k ir) { (* No Pending on Server side *)
-          if (!((   get_ir_test (oget s_smap.[b, j])
-                 \/ untested_partner_mod_s t c_smap = Some false)
-                /\ oget s_kp.[b] = None)) {
-            ek <- st.`2;
-            s_smap.[(b, j)] <- set_ir_eph (Accepted st t k ir);
-          }
-        }
-      }
-    end;
-    return ek;
-  }
-
-  proc c_test(i: int) : key option = {
-    var ks;
-    var k <- None;
-
-    if (tested = None) {
-      match c_smap.[i] with
-      | None => { }
-      | Some st => {
-          (* only accepted client instances that are not sesskey revealed, not ephkey revealed 
-             and not all partner instances are unfresh can be tested *)
-          if (st is Accepted st' t' k' ir') {
-            if (!(   get_ir_sess (oget c_smap.[i]) \/ get_ir_eph (oget c_smap.[i]) 
-                  \/ fresh_partner_mod_c t' s_smap s_kp = Some false)) {
-              if (b0 = false) {
-                k <- Some k';
-                c_smap.[i] <- set_ir_test (Accepted st' t' k' ir');
-              } else {
-                ks <$ dkey;
-                k <- Some ks;
-                c_smap.[i] <- set_ir_test (Accepted st' t' k' ir');
-              }
-              tested <- Some i;
-           }
-          }
-        }
-      end;
-    }
-    return k;
-  }
-
-  proc s_test(b: pkey, j: int) : key option = {
-    var ks;
-    var k <- None;
-
-    if (tested = None) {
-      match s_smap.[(b, j)] with
-      | None => { }
-      | Some st => {
-          (* only accepted server instances that are not sesskey revealed, not trivially broken
-             and not all partner instances are unfresh can be tested *)
-          if (st is Accepted st' t' k' ir') {
-            if (!(   get_ir_sess (oget s_smap.[b, j]) 
-                  \/ (get_ir_eph (oget s_smap.[b, j]) /\ s_kp.[b] = None)
-                  \/ fresh_partner_mod_s t' c_smap = Some false)) {
-              if (b0 = false) {
-                k <- Some k';
-                s_smap.[(b, j)] <- set_ir_test (Accepted st' t' k' ir');
-              } else {
-                ks <$ dkey;
-                k <- Some ks;
-                s_smap.[(b, j)] <- set_ir_test (Accepted st' t' k' ir');
-              }
-              tested <- Some (pick (get_fresh_partners_s t' GAKEb.c_smap));
-            }
-          }
-        }
-      end;
-    }
-    return k;
-  }
-}.
-
-
-(********************************************************************************)
-(* Adversary and Experiment for modified GAKE game *)
-module type A_GAKE_mod (O : GAKE_mod_out) = {
-  proc run() : bool
-}.
-
-module E_GAKE_mod (O: GAKE_mod_out_i) (A : A_GAKE_mod) = {
-
-  proc run(b: bool) : bool = {
-    var b' : bool;
-
-    O.init_mem(b);
-    
-    b' <@ A(O).run();
-    
-    return b';
-  }
-}.
-
-(* ------------------------------------------------------------------------------------------ *)
-(* Reduction preventing collisions and prediction of public keys  *)
-type server_state_mod = [
-  Honest_mod    of pkey
-| Corrupt_mod   of pkey
-| Dishonest_mod of pkey
-].
-
-op get_pkey_mod s_st =
-with s_st = Honest_mod    pk => pk
-with s_st = Corrupt_mod   pk => pk
-with s_st = Dishonest_mod pk => pk.
-
-op get_sr_mod s_st : bool =
-with s_st = Honest_mod    _ => false
-with s_st = Corrupt_mod   _ => true
-with s_st = Dishonest_mod _ => true.
-
-module (Meta_Red (A : A_GAKE) : A_GAKE_mod) (O : GAKE_mod_out) = {
-  module O_GAKE : GAKE_out = {
-    var unreg_ro : (pkey * pkey * s_id * pkey * pkey, (tag * key)) fmap
-
-    var servers : (s_id, server_state_mod) fmap
-    var pk_set : pkey fset
-  (*  var pred_ce : pkey fset
-    var pred_se : pkey fset*)
-    
-    var stop : bool
-
-    proc h(x : h_input) = {
-      var pk, tk;
-      var r <- (witness, witness);
-
-      if (!stop) {
-        if (x.`3 \in servers /\ !get_sr_mod (oget servers.[x.`3])) {
-          stop <- stop \/ x \in unreg_ro;
-          pk <- get_pkey_mod (oget servers.[x.`3]); 
-          r <@ O.h((x.`1, x.`2, pk, x.`4, x.`5));
-        } else {
-          tk <$ dtag `*` dkey;
-          if (x \notin unreg_ro) {
-            unreg_ro.[x] <- tk;
-          }
-          r <- oget unreg_ro.[x];
-        }
-
-        if (x.`4 \notin pk_set) {
-          pk_set <- pk_set `|` fset1 x.`4;
-        }
-        if (x.`5 \notin pk_set) {
-          pk_set <- pk_set `|` fset1 x.`5;
-        }
-      }
-
-      return r;
-    }
-
-    proc init_s(b: s_id) = {
-      var pk;
-      var r <- None;
-
-      if (!stop) {
-        if (b \notin servers) {
-          pk <@ O.init_s();
-          stop <- stop \/ pk \in pk_set;
-          servers.[b] <- Honest_mod pk;
-          pk_set <- pk_set `|` fset1 pk;
-
-        }
-        r <- Some (get_pkey_mod (oget servers.[b]));
-      }
-
-      return r;
-    }
-
-    proc set_cert(b: s_id, pk: pkey) = {
-      var r <- None;
-
-      if (!stop /\ b \notin servers) {
-        r <@ O.set_cert(pk);
-        servers.[b] <- Dishonest_mod pk;
-        pk_set <- pk_set `|` fset1 pk;
-      }
-
-      return r;
-    }
-
-    proc send_msg1(i: int, m1: s_id) = {
-      var pk; 
-      var r <- None;
-
-      if (!stop /\ m1 \in servers) {
-        pk <- get_pkey_mod (oget servers.[m1]);
-        r <@ O.send_msg1(i, pk);
-       if (r <> None) {
-         stop <- stop \/ (oget r \in pk_set);
-         pk_set <- pk_set `|` fset1 (oget r);
-       }
-      }
-
-      return r;
-    }
-
-    proc send_msg2(b: s_id, j: int, m2: pkey) = {
-      var pk; 
-      var r <- None;
-
-      if (!stop /\ b \in servers) {
-        if (m2 \notin pk_set) {
-          pk_set <- pk_set `|` fset1 m2;
-        }
-
-        pk <- get_pkey_mod (oget servers.[b]);
-        r <@ O.send_msg2(pk, j, m2);
-        if (r <> None) {
-          stop <- stop \/ ((oget r).`1 \in pk_set);
-          pk_set <- pk_set `|` fset1 (oget r).`1;  
-        }
-      }
-
-      return r;
-    }
-
-    proc send_msg3(i: int, m3: pkey * tag) = {
-      var r <- None;
-
-      if (!stop) {
-         if (m3.`1 \notin pk_set) {
-           pk_set <- pk_set `|` fset1 m3.`1;
-         }
-
-         r <@ O.send_msg3(i, m3);
-      }
-
-      return r;
-    }
-
-    proc c_rev_skey(i: int) = {
-      var r <- None;
-
-      if (!stop) {
-        r <@ O.c_rev_skey(i);
-      }
-
-      return r;
-    }
-
-    proc s_rev_skey(b: s_id, j: int) = {
-      var pk;
-      var r <- None;
-
-      if (!stop /\ b \in servers) {
-        pk <- get_pkey_mod (oget servers.[b]);
-        r <@ O.s_rev_skey(pk, j);
-      }
-
-      return r;     
-    }
-
-    proc rev_ltkey(b: s_id) = {
-      var pk;
-      var r <- None;
-
-      if (!stop /\ b \in servers) {
-        pk <- get_pkey_mod (oget servers.[b]);
-        r <@ O.rev_ltkey(pk);
-        if (r <> None) {
-          servers.[b] <- Corrupt_mod pk;
-        }
-      }
-
-      return r;
-    }
-
-    proc c_rev_ephkey(i : int) = {
-      var r <- None;
-
-      if (!stop) {
-        r <@ O.c_rev_ephkey(i);
-      }
-
-      return r;
-    }
-
-    proc s_rev_ephkey(b: s_id, j: int) = {
-      var pk;
-      var r <- None;
-
-      if (!stop /\ b \in servers) {
-        pk <- get_pkey_mod (oget servers.[b]);
-        r <@ O.s_rev_ephkey(pk, j);
-      }
-
-      return r;     
-    }
-
-    proc c_test(i : int) = {
-      var r <- None;
-
-      if (!stop) {
-        r <@ O.c_test(i);
-      }
-
-      return r;
-    }
-
-    proc s_test(b: s_id, j: int) = {
-      var pk;
-      var r <- None;
-
-      if (!stop /\ b \in servers) {
-        pk <- get_pkey_mod (oget servers.[b]);
-        r <@ O.s_test(pk, j);
-      }
-
-      return r;
-    }
-  }
-
-  proc run() : bool = {
-    var b';
-
-    O_GAKE.unreg_ro <- empty;
-    O_GAKE.servers <- empty;
-    O_GAKE.pk_set <- fset0;
-    O_GAKE.stop <- false;
-
-    b' <@ A(O_GAKE).run();
-
-    return b';
-  }
-}.
-
 
 (* Introduce stop in original game *)
 module GAKEb_st (S: Server) (C: Client) (H : HROc.RO) = {
@@ -1112,13 +446,265 @@ module GAKEb_st (S: Server) (C: Client) (H : HROc.RO) = {
 
 
 (* ------------------------------------------------------------------------------------------ *)
+(* Modified game without server ids *)
+clone import GAKE_nosid as GAKE_mod with 
+  type trace <- trace,
+  type pkey <- pkey,
+  type skey <- skey,
+  type key <- key,
+  type tag <- tag,
+  type pr_st_client <- pr_st_client_mod,
+  type pr_st_server <- pr_st_server_mod,
+  op dskey <- dt,
+  op dkey <- dkey,
+  op dtag <- dtag.
+
+
+(* ------------------------------------------------------------------------------------------ *)
+(* Reduction preventing collisions and prediction of public keys  *)
+type server_state_mod = [
+  Inner of pkey
+| Outer of pkey
+].
+
+op get_pkey_mod s_st =
+with s_st = Inner pk => pk
+with s_st = Outer pk => pk.
+
+op get_sr_mod s_st : bool =
+with s_st = Inner _ => false
+with s_st = Outer _ => true.
+
+print GAKEc.GAKE_out.
+
+module (Meta_Red (A : GAKEc.A_GAKE) : GAKE_mod.A_GAKE) (O : GAKE_mod.GAKE_out) = {
+  module O_GAKE : GAKEc.GAKE_out = {
+    var unreg_ro : (pkey * pkey * s_id * pkey * pkey, (tag * key)) fmap
+
+    var servers : (s_id, server_state_mod) fmap
+    var pk_set : pkey fset
+  (*  var pred_ce : pkey fset
+    var pred_se : pkey fset*)
+    
+    var stop : bool
+
+    proc h(x : GAKEc.h_input) = {
+      var pk, tk;
+      var r <- (witness, witness);
+
+      if (!stop) {
+        if (x.`3 \in servers /\ !get_sr_mod (oget servers.[x.`3])) {
+          stop <- stop \/ x \in unreg_ro;
+          pk <- get_pkey_mod (oget servers.[x.`3]); 
+          r <@ O.h((x.`1, x.`2, pk, x.`4, x.`5));
+        } else {
+          tk <$ dtag `*` dkey;
+          if (x \notin unreg_ro) {
+            unreg_ro.[x] <- tk;
+          }
+          r <- oget unreg_ro.[x];
+        }
+
+        if (x.`4 \notin pk_set) {
+          pk_set <- pk_set `|` fset1 x.`4;
+        }
+        if (x.`5 \notin pk_set) {
+          pk_set <- pk_set `|` fset1 x.`5;
+        }
+      }
+
+      return r;
+    }
+
+    proc init_s(b : s_id): pkey option = {
+      var pko;
+      var r <- None;
+
+      if (!stop) {
+        if (b \notin servers) {
+          pko <@ O.init_s();
+          if (pko is Some pk) {
+            stop <- stop \/ pk \in pk_set;
+            servers.[b] <- Inner pk;
+          }
+        }
+        r <- Some (get_pkey_mod (oget servers.[b]));
+      }
+      return r;
+    }
+
+    proc set_cert(b: s_id, pk: pkey) = {
+      var r <- None;
+
+      if (!stop /\ b \notin servers) {
+        servers.[b] <- Outer pk;
+        pk_set <- pk_set `|` fset1 pk;
+        r <- Some ();
+      }
+
+      return r;
+    }
+
+    proc send_msg1(i: int, m1: s_id) = {
+      var pk; 
+      var r <- None;
+
+      if (!stop /\ m1 \in servers) {
+        pk <- get_pkey_mod (oget servers.[m1]);
+        r <@ O.send_msg1(i, pk);
+       if (r <> None) {
+         stop <- stop \/ (oget r \in pk_set);
+         pk_set <- pk_set `|` fset1 (oget r);
+       }
+      }
+
+      return r;
+    }
+
+    proc send_msg2(b: s_id, j: int, m2: pkey) = {
+      var pk; 
+      var r <- None;
+
+      if (!stop /\ b \in servers) {
+        if (m2 \notin pk_set) {
+          pk_set <- pk_set `|` fset1 m2;
+        }
+
+        pk <- get_pkey_mod (oget servers.[b]);
+        r <@ O.send_msg2(pk, j, m2);
+        if (r <> None) {
+          stop <- stop \/ ((oget r).`1 \in pk_set);
+          pk_set <- pk_set `|` fset1 (oget r).`1;  
+        }
+      }
+
+      return r;
+    }
+
+    proc send_msg3(i: int, m3: pkey * tag) = {
+      var r <- None;
+
+      if (!stop) {
+         if (m3.`1 \notin pk_set) {
+           pk_set <- pk_set `|` fset1 m3.`1;
+         }
+
+         r <@ O.send_msg3(i, m3);
+      }
+
+      return r;
+    }
+
+    proc c_rev_skey(i: int) = {
+      var r <- None;
+
+      if (!stop) {
+        r <@ O.c_rev_skey(i);
+      }
+
+      return r;
+    }
+
+    proc s_rev_skey(b: s_id, j: int) = {
+      var pk;
+      var r <- None;
+
+      if (!stop /\ b \in servers) {
+        pk <- get_pkey_mod (oget servers.[b]);
+        r <@ O.s_rev_skey(pk, j);
+      }
+
+      return r;     
+    }
+
+    proc rev_ltkey(b: s_id) = {
+      var pk;
+      var r <- None;
+
+      if (!stop /\ b \in servers) {
+        pk <- get_pkey_mod (oget servers.[b]);
+        r <@ O.rev_ltkey(pk);
+        if (r <> None) {
+          servers.[b] <- Outer pk; (* Do I need to know that this was honest before? *)
+        }
+      }
+
+      return r;
+    }
+
+    proc c_rev_ephkey(i : int) = {
+      var r <- None;
+
+      if (!stop) {
+        r <@ O.c_rev_ephkey(i);
+      }
+
+      return r;
+    }
+
+    proc s_rev_ephkey(b: s_id, j: int) = {
+      var pk;
+      var r <- None;
+
+      if (!stop /\ b \in servers) {
+        pk <- get_pkey_mod (oget servers.[b]);
+        r <@ O.s_rev_ephkey(pk, j);
+      }
+
+      return r;     
+    }
+
+    proc c_test(i : int) = {
+      var r <- None;
+
+      if (!stop) {
+        r <@ O.c_test(i);
+      }
+
+      return r;
+    }
+
+    proc s_test(b: s_id, j: int) = {
+      var pk;
+      var r <- None;
+
+      if (!stop /\ b \in servers) {
+        if (! get_sr_mod (oget servers.[b])) {
+          pk <- get_pkey_mod (oget servers.[b]);
+          r <@ O.s_test(pk, j);
+        }
+      }
+
+      return r;
+    }
+  }
+
+  proc run() : bool = {
+    var b';
+
+    O_GAKE.unreg_ro <- empty;
+    O_GAKE.servers <- empty;
+    O_GAKE.pk_set <- fset0;
+    O_GAKE.stop <- false;
+
+    b' <@ A(O_GAKE).run();
+
+    return b';
+  }
+}.
+
+
+
+
+
+(* ------------------------------------------------------------------------------------------ *)
 (* Security Proof *)
 (* ------------------------------------------------------------------------------------------ *)
 section.
 
-declare module A <: A_GAKE {-RO, -HROc.RO, -Meta_Red, -GAKEb, -GAKEb_st, -GAKEb_mod }.
+declare module A <: GAKEc.A_GAKE {-RO, -GAKEc.HROc.RO, -Meta_Red, -GAKEc.GAKEb, -GAKEb_st, -GAKE_mod.GAKEb }.
 
-declare axiom A_ll (G <: GAKE_out{-A}):
+declare axiom A_ll (G <: GAKEc.GAKE_out{-A}):
   islossless G.h =>
   islossless G.init_s =>
   islossless G.set_cert =>
@@ -1135,67 +721,51 @@ declare axiom A_ll (G <: GAKE_out{-A}):
   islossless A(G).run.
 
 
-lemma gake_st bit &m: Pr[E_GAKE(GAKEb(NTOR_S(HROc.RO), NTOR_C(HROc.RO), HROc.RO), A).run(bit) @ &m : res] =  Pr[E_GAKE(GAKEb_st(NTOR_S(HROc.RO), NTOR_C(HROc.RO), HROc.RO), A).run(bit) @ &m : res].
+lemma gake_st bit &m: Pr[GAKEc.E_GAKE(GAKEc.GAKEb(NTOR_S(GAKEc.HROc.RO), NTOR_C(GAKEc.HROc.RO), GAKEc.HROc.RO), A).run(bit) @ &m : res] =  Pr[GAKEc.E_GAKE(GAKEb_st(NTOR_S(GAKEc.HROc.RO), NTOR_C(GAKEc.HROc.RO), GAKEc.HROc.RO), A).run(bit) @ &m : res].
 proof.
 byequiv => //.
 proc; inline.
-call (: ={b0, servers, c_smap, s_smap, tested}(GAKEb, GAKEb_st) /\ ={m}(HROc.RO, HROc.RO)); try sim />.
+call (: ={b0, servers, c_smap, s_smap, tested}(GAKEc.GAKEb, GAKEb_st) /\ ={m}(GAKEc.HROc.RO, GAKEc.HROc.RO)); try sim />.
 
 + proc; inline.
   auto => />.
 qed.
 
-
-op rem_sid_c (s : pr_st_client instance_state) : pr_st_client_mod instance_state =
-match s with 
-| Pending st pt ir => Pending (st.`2, st.`3) pt ir
-| Accepted st t k ir => Accepted (st.`2, st.`3) t k ir
-| Aborted st t ir => Aborted (Some ((oget st).`2, (oget st).`3)) t ir
-end.
-
-op rem_sid_s (s : pr_st_server instance_state) : pr_st_server_mod instance_state =
-match s with 
-| Pending st pt ir => Pending (st.`2, st.`3) pt ir
-| Accepted st t k ir => Accepted (st.`2, st.`3) t k ir
-| Aborted st t ir => Aborted (Some ((oget st).`2, (oget st).`3)) t ir
-end.
-
-lemma gake_st_mod bit &m: `| Pr[E_GAKE(GAKEb_st(NTOR_S(HROc.RO), NTOR_C(HROc.RO), HROc.RO), A).run(bit) @ &m : res] - Pr[E_GAKE_mod(GAKEb_mod(NTOR_S_mod(RO), NTOR_C_mod(RO), RO), Meta_Red(A)).run(bit) @ &m : res] | <= Pr[E_GAKE(GAKEb_st(NTOR_S(HROc.RO), NTOR_C(HROc.RO), HROc.RO), A).run(bit) @ &m : GAKEb_st.stop].
+lemma gake_st_mod bit &m: `| Pr[GAKEc.E_GAKE(GAKEb_st(NTOR_S(GAKEc.HROc.RO), NTOR_C(GAKEc.HROc.RO), GAKEc.HROc.RO), A).run(bit) @ &m : res] - Pr[GAKE_mod.E_GAKE(GAKE_mod.GAKEb(NTOR_S_mod(RO), NTOR_C_mod(RO), RO), Meta_Red(A)).run(bit) @ &m : res] | <= Pr[GAKEc.E_GAKE(GAKEb_st(NTOR_S(GAKEc.HROc.RO), NTOR_C(GAKEc.HROc.RO), GAKEc.HROc.RO), A).run(bit) @ &m : GAKEb_st.stop].
 proof.
 rewrite StdOrder.RealOrder.distrC.
 byequiv (: _ ==> _) : Meta_Red.O_GAKE.stop => //; first last.
 + smt().
 symmetry; proc; inline*.
 wp; call (: Meta_Red.O_GAKE.stop
-          , ={b0, tested}(GAKEb_st, GAKEb_mod) /\ ={pk_set, stop}(GAKEb_st, Meta_Red.O_GAKE)
-               /\ (forall x, x \in HROc.RO.m{1} => x.`3 \in Meta_Red.O_GAKE.servers{2} => x \notin Meta_Red.O_GAKE.unreg_ro{2}
-                    => HROc.RO.m{1}.[x] = RO.m{2}.[(x.`1, x.`2, get_pkey_mod (oget Meta_Red.O_GAKE.servers{2}.[x.`3]), x.`4, x.`5)])
-               /\ (forall x, x \in HROc.RO.m{1} => x.`3 \notin Meta_Red.O_GAKE.servers{2} \/ get_sr_mod (oget Meta_Red.O_GAKE.servers{2}.[x.`3])
-                    => HROc.RO.m{1}.[x] =  Meta_Red.O_GAKE.unreg_ro{2}.[x])
-               /\ (forall x, x \notin HROc.RO.m{1} => x.`3 \in Meta_Red.O_GAKE.servers{2} => !get_sr_mod (oget Meta_Red.O_GAKE.servers{2}.[x.`3])
+          , ={b0, tested}(GAKEb_st, GAKE_mod.GAKEb) /\ ={pk_set, stop}(GAKEb_st, Meta_Red.O_GAKE)
+               /\ (forall x, x \in GAKEc.HROc.RO.m{1} => x.`3 \in Meta_Red.O_GAKE.servers{2} => x \notin Meta_Red.O_GAKE.unreg_ro{2}
+                    => GAKEc.HROc.RO.m{1}.[x] = RO.m{2}.[(x.`1, x.`2, get_pkey_mod (oget Meta_Red.O_GAKE.servers{2}.[x.`3]), x.`4, x.`5)])
+               /\ (forall x, x \in GAKEc.HROc.RO.m{1} => x.`3 \notin Meta_Red.O_GAKE.servers{2} \/ get_sr_mod (oget Meta_Red.O_GAKE.servers{2}.[x.`3])
+                    => GAKEc.HROc.RO.m{1}.[x] =  Meta_Red.O_GAKE.unreg_ro{2}.[x])
+               /\ (forall x, x \notin GAKEc.HROc.RO.m{1} => x.`3 \in Meta_Red.O_GAKE.servers{2} => !get_sr_mod (oget Meta_Red.O_GAKE.servers{2}.[x.`3])
                     => (x.`1, x.`2, get_pkey_mod (oget Meta_Red.O_GAKE.servers{2}.[x.`3]), x.`4, x.`5) \notin RO.m{2})
-               /\ (forall x, x \notin HROc.RO.m{1} => x \notin  Meta_Red.O_GAKE.unreg_ro{2})
+               /\ (forall x, x \notin GAKEc.HROc.RO.m{1} => x \notin  Meta_Red.O_GAKE.unreg_ro{2})
                /\ (forall b1 b2, b1 \in Meta_Red.O_GAKE.servers{2} => b2 \in Meta_Red.O_GAKE.servers{2} 
                     => !get_sr_mod (oget Meta_Red.O_GAKE.servers{2}.[b1])
-                    => oget Meta_Red.O_GAKE.servers{2}.[b1] = oget Meta_Red.O_GAKE.servers{2}.[b2] 
+                    => oget Meta_Red.O_GAKE.servers{2}.[b1] = oget Meta_Red.O_GAKE.servers{2}.[b2]
                     => b1 = b2)
-               /\ (forall i, i \in GAKEb_st.c_smap{1} <=> i \in GAKEb_mod.c_smap{2})
-               /\ (forall i, i \in GAKEb_st.c_smap{1} => rem_sid_c (oget GAKEb_st.c_smap{1}.[i]) = oget GAKEb_mod.c_smap{2}.[i])
-               /\ (forall b j, (b, j) \in GAKEb_st.s_smap{1} => b \in Meta_Red.O_GAKE.servers{2}
+               /\ (forall i, i \in GAKEb_st.c_smap{1} <=> i \in GAKE_mod.GAKEb.c_smap{2})
+               /\ (forall i, i \in GAKEb_st.c_smap{1} => rem_sid_c (oget GAKEb_st.c_smap{1}.[i]) = oget GAKE_mod.GAKEb.c_smap{2}.[i])
+               /\ (forall b j, (b, j) \in GAKEb_st.s_smap{1} => b \in Meta_Red.O_GAKE.servers{2} /\ !get_sr_mod (oget Meta_Red.O_GAKE.servers{2}.[b])
                                       /\ (get_pkey_mod (oget Meta_Red.O_GAKE.servers{2}.[b]), j) \in GAKEb_mod.s_smap{2}
                                       /\ rem_sid_s (oget GAKEb_st.s_smap{1}.[(b, j)]) = oget GAKEb_mod.s_smap{2}.[(get_pkey_mod (oget Meta_Red.O_GAKE.servers{2}.[b]), j)])
                /\ (forall b j, (b, j) \notin GAKEb_st.s_smap{1} => b \in Meta_Red.O_GAKE.servers{2} => !get_sr_mod (oget Meta_Red.O_GAKE.servers{2}.[b])
                     => (get_pkey_mod (oget Meta_Red.O_GAKE.servers{2}.[b]), j) \notin GAKEb_mod.s_smap{2})
-               /\ (forall b j, (get_pkey_mod (oget Meta_Red.O_GAKE.servers{2}.[b]), j) \in GAKEb_mod.s_smap{2} => get_sr_mod (oget Meta_Red.O_GAKE.servers{2}.[b])
-                    => (exists b2, get_pkey_mod (oget Meta_Red.O_GAKE.servers{2}.[b]) = get_pkey_mod (oget Meta_Red.O_GAKE.servers{2}.[b2])
-                                      /\ !get_sr_mod (oget Meta_Red.O_GAKE.servers{2}.[b2])))
                /\ (forall x, x \in GAKEb_st.unreg_ro{1} <=> x \in Meta_Red.O_GAKE.unreg_ro{2})
                /\ (forall b, b \in GAKEb_st.servers{1} <=> b \in Meta_Red.O_GAKE.servers{2})
                /\ (forall b, b \in GAKEb_st.servers{1} => get_pkey (oget GAKEb_st.servers{1}.[b]) = get_pkey_mod (oget Meta_Red.O_GAKE.servers{2}.[b])
                                       /\ get_sr_ltk (oget GAKEb_st.servers{1}.[b]) = get_sr_mod (oget Meta_Red.O_GAKE.servers{2}.[b]))
                /\ (forall pk x1 x2 x4 x5, pk \notin GAKEb_mod.s_kp{2} => !rng Meta_Red.O_GAKE.servers{2} (Honest_mod pk) /\ (x1, x2, pk, x4, x5) \notin RO.m{2})
-               /\ (forall b, b \in Meta_Red.O_GAKE.servers{2} => get_pkey_mod (oget Meta_Red.O_GAKE.servers{2}.[b]) \in GAKEb_mod.s_kp{2})
-               /\ (forall pk j, pk \notin Meta_Red.O_GAKE.pk_set{2} => pk \notin GAKEb_mod.s_kp{2} /\ (pk, j) \notin GAKEb_mod.s_smap{2})
+               /\ (forall b, b \in Meta_Red.O_GAKE.servers{2} => get_pkey_mod (oget Meta_Red.O_GAKE.servers{2}.[b]) \in GAKEb_mod.s_pk{2})
+               /\ (forall b, b \in Meta_Red.O_GAKE.servers{2} => !get_sr_mod (oget Meta_Red.O_GAKE.servers{2}.[b])
+                    => obind get_skey GAKEb_st.servers{1}.[b] = oget GAKEb_mod.s_kp{2}.[get_pkey_mod (oget Meta_Red.O_GAKE.servers{2}.[b])])
+               /\ (forall pk j, pk \notin Meta_Red.O_GAKE.pk_set{2} => pk \notin GAKEb_mod.s_kp{2} /\ pk \notin GAKEb_mod.s_pk{2} /\ (pk, j) \notin GAKEb_mod.s_smap{2})
           , GAKEb_st.stop{1} = Meta_Red.O_GAKE.stop{2}) => //.
 
 - exact A_ll.
@@ -1226,14 +796,7 @@ wp; call (: Meta_Red.O_GAKE.stop
   sp; if {2} => //.
   + if => //.
     + auto => />. smt().
-    + auto => /> &1 &2 ? ? ? ? ? ? ? ? ? ? inv ? ? ? ? ? ? ? sk *. split. smt(mem_set get_setE in_fsetU in_fset1). split. smt(mem_set get_setE in_fsetU in_fset1). split. smt(mem_set get_setE in_fsetU in_fset1). split. smt(mem_set get_setE in_fsetU in_fset1). split. smt(mem_set get_setE in_fsetU in_fset1). split. smt(mem_set get_setE in_fsetU in_fset1). split. smt(mem_set get_setE in_fsetU in_fset1). split. 
-move => b0 j.
-case (b0 = b{2}) => b0eq.
-admit. 
-rewrite get_set_neqE //=.
-move =>  insm nh.
-have := inv b0 j insm nh. 
-smt(mem_set get_setE in_fsetU in_fset1). smt(mem_set get_setE in_fsetU in_fset1).
+    + auto => /> &1 &2 *. smt(mem_set get_setE in_fsetU in_fset1).
     auto => /> &1 &2 *. 
     smt().
   if {1} => //; auto => />.
@@ -1241,13 +804,10 @@ smt(mem_set get_setE in_fsetU in_fset1). smt(mem_set get_setE in_fsetU in_fset1)
   by rewrite dt_ll bad //=.
 - move => &1; proc; inline.
   rcondf ^if; auto => />.
-                
+
 - proc; inline.
   sp 1 1; if {2} => //.
-  auto => /> &1 &2 *. split. smt(mem_set get_setE in_fsetU in_fset1). move => *. split. smt(mem_set get_setE in_fsetU in_fset1). split. smt(mem_set get_setE in_fsetU in_fset1). split. smt(mem_set get_setE in_fsetU in_fset1). split. smt(mem_set get_setE in_fsetU in_fset1). split. smt(mem_set get_setE in_fsetU in_fset1). split. smt(mem_set get_setE in_fsetU in_fset1). split. 
-
-
-smt(mem_set get_setE in_fsetU in_fset1).
+  + auto => /> &1 &2 *. smt(mem_set get_setE in_fsetU in_fset1).
   auto => /> &1 &2 *. smt().
 - move => &2 bad; proc; inline. auto => />.
 - move => &1; proc; inline.
@@ -1282,7 +842,7 @@ smt(mem_set get_setE in_fsetU in_fset1).
 - proc; inline.
   sp 1 1; if {2} => //.
   + sp 1 0; if => //.
-    + sp 1 7. match = => //. 
+    + sp 1 7. match.  
       + auto => /> &1 &2 *. admit.
       + auto => />. smt(get_setE mem_set in_fsetU in_fset1).
       auto => />. smt(get_setE mem_set in_fsetU in_fset1).
@@ -1446,34 +1006,25 @@ smt(mem_set get_setE in_fsetU in_fset1).
 
 - proc; inline.
   sp 1 1; if {2} => //.
-  + sp. if => //.
-    + match.
-      + move => /> &1 &2 ? ? ? ? ? ? ? ? ? inv *.
-        split. smt(). smt().
-        do rewrite -domNE.
-        case (get_sr_mod (oget Meta_Red.O_GAKE.servers{2}.[b{2}])); 2: by smt().
-
-        smt().
-     
-        + have := inv b{2} j{2}.
-
-      + match None {2} ^match.
-       
+  + sp. if {2} => //. 
+    + sp; if => //.
+      + match; 1..2: smt().
+        + auto => />.
+        + move => stl str.
+          + match; 1..3: smt().
+            + move => sl ptl irl sr ptr irr.
+              auto => />.
+            + move => sl tl kl irl sr tr kr irr.
+              if => //.
+              + auto => /> &1 &2 *. admit. (* relate fresh partner and such *)
+              if => //.
+              + auto => />. admit.
+              auto => />. admit.
+            auto => />.
+          auto => />.
         auto => />.
-      match Some {2} ^match. admit.
-      match {1} => //.
-      + match Pending {2} ^match. auto => /#.
-        auto => />.
-      + match Accepted {2} ^match. auto => /#.
-        if => //. 
-        + auto => /> &1 &2 *. admit. (* relate fresh partner and such *)
-        + if => //. 
-          + auto => />. admit.
-          auto => />. admit.
-        auto => />.
-      match Aborted {2} ^match. auto => /#.
-      auto => />.
-    auto => />.
+      if {1} => //.
+      match {1} => //. admit. (* when in state1 then honest *)
   if {1} => //; match {1} => //. 
   match {1} => //; if {1} => //.
   if {1} => //; auto => />; smt(get_setE mem_set in_fsetU in_fset1).
